formalization/thesis/Isotope/LambdaSSA/Subtyping/LocallyNameless/ToDeBruijn/Typing.lean
@@ -1,0 +1,52 @@
+import Isotope.LambdaSSA.LocallyNameless.ToDeBruijn.Typing
+import Isotope.LambdaSSA.Subtyping.LocallyNameless.Typing
+import Isotope.LambdaSSA.Subtyping.Typing
+
+namespace Isotope.LambdaSSA.Subtyping.LocallyNameless.ToDeBruijn
+
+open Isotope.LambdaSSA
+open Isotope.LambdaSSA.LocallyNameless.ToDeBruijn
+
+noncomputable def eraseTm_hasType [LambdaIter.TypeFormers τ] [LambdaIter.Subtyping τ]
+    [LambdaIter.HasTy Φ τ]
+    {β : LambdaSSA.LocallyNameless.BoundCtx τ n}
+    {t : LambdaSSA.LocallyNameless.Tm Empty Φ n}
+    (h : Subtyping.LocallyNameless.Tm.HasType Φ
+      (LambdaIter.Ctx.nil : LambdaIter.Ctx Empty τ) β t A) :
+    Subtyping.Tm.HasType (context β) (eraseTm t) A := by
+  induction h with
+  | fv h => cases h
+  | bv => exact .var (getElem_context _ _)
+  | op _ ih => exact .op ih
+  | let₁ _ _ iha ihb => exact .let₁ iha ihb
+  | pair _ _ iha ihb => exact .pair iha ihb
+  | unit => exact .unit
+  | let₂ _ _ iha ihb => exact .let₂ iha ihb
+  | inl _ ih => exact .inl ih
+  | inr _ ih => exact .inr ih
+  | case _ _ _ ihe ihl ihr => exact .case ihe ihl ihr
+  | abort _ ih => exact .abort ih
+  | sub _ d ih => exact .sub ih d
+
+noncomputable def eraseRegion_hasType [LambdaIter.TypeFormers τ] [LambdaIter.Subtyping τ]
+    [LambdaIter.HasTy Φ τ]
+    {β : LambdaSSA.LocallyNameless.BoundCtx τ n}
+    {δ : LambdaSSA.LocallyNameless.BoundCtx τ l}
+    {r : LambdaSSA.LocallyNameless.Region Empty Empty Φ n l}
+    (h : Subtyping.LocallyNameless.Region.HasType Φ
+      (LambdaIter.Ctx.nil : LambdaIter.Ctx Empty τ)
+      (LambdaIter.Ctx.nil : LambdaIter.Ctx Empty τ) β δ r) :
+    Subtyping.Region.HasType (context β) (eraseRegion r) (context δ) := by
+  induction h with
+  | br_free h => cases h
+  | br_bound harg => exact .br (getElem_context _ _) (eraseTm_hasType harg)
+  | case hdiscr _ _ ihr ihs => exact .case (eraseTm_hasType hdiscr) ihr ihs
+  | let₁ hvalue _ ihr => exact .let₁ (eraseTm_hasType hvalue) ihr
+  | let₂ hvalue _ ihr => exact .let₂ (eraseTm_hasType hvalue) ihr
+  | cfg R _ _ ihe ihbs =>
+      apply Subtyping.Region.HasType.cfg R
+      · simpa using ihe
+      · intro i
+        simpa using ihbs i
+
+end Isotope.LambdaSSA.Subtyping.LocallyNameless.ToDeBruijn
