formalization/thesis/Isotope/LambdaSSA/Subtyping/Named.lean
@@ -1,0 +1,2 @@
+import Isotope.LambdaSSA.Subtyping.Named.Typing
+import Isotope.LambdaSSA.Subtyping.Named.ToLocallyNameless.Typing
