formalization/thesis/Isotope/LambdaSeq/Subtyping.lean
@@ -1,5 +1,6 @@
 import Isotope.LambdaSeq.Typing
 import Isotope.LambdaSeq.Semantics
 import Isotope.LambdaSeq.Subtyping.Semantics.Named
+import Isotope.LambdaSeq.Subtyping.Semantics.Categorical.Chosen
 
 /-! # Proof-relevant subtyping variant of lambda-seq -/
